Try to copy imp-in-lean in Basic

LeanTmp/Basic.lean
@@ -1,1 +1,343 @@
-def hello := "world"
+import Mathlib.Data.Real.Basic
+import Mathlib.Data.Finsupp.AList
+
+def total_map (A : Type) := String -> A
+
+def t_empty {A: Type} (v: A) : total_map A :=
+(fun _ => v)
+
+def t_update {A: Type}(m: total_map A)(x: String)(v :A) :=
+  fun y => if (x == y) then v else (m y)
+
+notation:max "!->" v => (t_empty v)
+notation:max x "!->" v ";" m => (t_update m x v)
+
+def ex_map := "y" !-> 6; ("x" !-> 3; (!-> 0))
+
+#eval (t_update ex_map "x" 4) "x"
+
+def state := total_map Nat
+
+namespace no_state
+inductive aexp where
+  | ANum (n : Nat)
+  | APlus (a1 a2 : aexp)
+  | AMinus (a1 a2 : aexp)
+  | AMult (a1 a2 : aexp)
+
+open aexp -- open namespace
+#check (APlus (ANum 3))
+
+inductive bexp where
+  | BTrue
+  | BFalse
+  | BEq (a1 a2 : aexp)
+  | BNeq (a1 a2 : aexp)
+  | BLe (a1 a2 : aexp)
+  | BGt (a1 a2 : aexp)
+  | BNot (b : bexp)
+  | BAnd (b1 b2 : bexp)
+
+open bexp
+#check BTrue
+#check (BEq (ANum 3) (ANum 3))
+
+------------- Evaluation as functions ----------------------
+
+def aeval (a : aexp) : Nat :=
+  match a with
+  | ANum n => n
+  | APlus  a1 a2 => (aeval a1) + (aeval a2)
+  | AMinus a1 a2 => (aeval a1) - (aeval a2)
+  | AMult  a1 a2 => (aeval a1) * (aeval a2)
+
+def beval (b : bexp) : Bool :=
+  match b with
+  | BTrue       => true
+  | BFalse      => false
+  | bexp.BEq a1 a2   => (aeval a1) = (aeval a2)
+  | BNeq a1 a2  => ¬ ((aeval a1) = (aeval a2))
+  | BLe a1 a2   => (aeval a1) <= (aeval a2)
+  | BGt a1 a2   => ¬ ((aeval a1) <= (aeval a2))
+  | BNot b1     => ¬ (beval b1)
+  | BAnd b1 b2  =>  (beval b1) ∧ (beval b2)
+
+
+
+---------------- Evaluation as a Relation ----------------------
+
+inductive aevalR : aexp -> Nat -> Prop where
+  | E_ANum (n : Nat) :
+      aevalR (ANum n) n
+  | E_APlus (e1 e2 : aexp) (n1 n2 : Nat)
+      (H1 : aevalR e1 n1)
+      (H2 : aevalR e2 n2) :
+      aevalR (APlus e1 e2) (n1 + n2)
+  | E_AMinus (e1 e2 : aexp) (n1 n2 : Nat)
+      (H1 : aevalR e1 n1)
+      (H2 : aevalR e2 n2) :
+      aevalR (AMinus e1 e2) (n1 - n2)
+  | E_AMult (e1 e2 : aexp) (n1 n2 : Nat)
+      (H1 : aevalR e1 n1)
+      (H2 : aevalR e2 n2) :
+      aevalR (AMult e1 e2) (n1 * n2)
+
+inductive bevalR: bexp -> Bool -> Prop where
+  | E_BTrue : bevalR BTrue true
+  | E_BFalse : bevalR BFalse false
+  | E_BEq : ∀ (a1 a2 : aexp) (n1 n2 : Nat),
+      (aevalR a1 n1) ->
+      (aevalR a2 n2) ->
+      bevalR (BEq a1 a2) (n1 = n2)
+  | E_BNeq : ∀ (a1 a2 : aexp) (n1 n2 : Nat),
+    (aevalR a1 n1) ->
+    (aevalR a2 n2) ->
+    bevalR (BNeq a1 a2) (¬ (n1 = n2))
+  | E_BLe : ∀ (a1 a2 : aexp) (n1 n2 : Nat),
+    (aevalR a1 n1) ->
+    (aevalR a2 n2) ->
+    bevalR (BLe a1 a2) (n1 <= n2)
+  | E_BGt : ∀ (a1 a2 : aexp) (n1 n2 : Nat),
+    (aevalR a1 n1) ->
+    (aevalR a2 n2) ->
+    bevalR (BGt a1 a2) (¬ (n1 <= n2))
+  | E_BNot : ∀ (b : bexp) (b' : Bool),
+    (bevalR b b') ->
+    bevalR (BNot b) (¬b')
+  | E_BAnd : ∀ (b1 b2 : bexp) (b1' b2' : Bool),
+    (bevalR b1 b1') ->
+    (bevalR b2 b2') ->
+    bevalR (BAnd b1 b2) (and b1' b2')
+
+-- Add notation
+infixl:65   " ==> " => aevalR  -- left-associative
+infixl:65   " ==>b " => bevalR  -- left-associative
+
+---------  Equivalence of evaluation as functions vs relations ------------
+
+theorem aeval_iff_aevalR : ∀ a n, (a ==> n) <-> aeval a = n := by
+  intros a n
+  constructor
+  · intros H
+    induction H <;> try
+      {rw [aeval]; rename_i H1_ih H2_ih; rw [H1_ih]; rw [H2_ih]}
+    rfl
+  . revert n; induction a <;> intros n H;
+    case mpr.ANum n =>
+      rw [aeval.eq_def] at H; simp at H; rewrite [H]; constructor
+    case mpr.APlus a1_ih a2_ih =>
+      rw [<- H]; rw [aeval]; apply aevalR.E_APlus;
+      apply a1_ih; rfl; apply a2_ih; rfl
+    case mpr.AMinus a1_ih a2_ih =>
+      rw [<- H]; rw [aeval]; apply aevalR.E_AMinus;
+      apply a1_ih; rfl; apply a2_ih; rfl
+    case mpr.AMult a1_ih a2_ih =>
+      rw [<- H]; rw [aeval]; apply aevalR.E_AMult;
+      apply a1_ih; rfl; apply a2_ih; rfl
+
+theorem beval_iff_bevalR : ∀ b bv, b ==>b bv <-> beval b = bv := by
+  intros b bv
+  constructor
+  . intros H
+    induction H
+      -- 2 IH on arithmetic operands (le, gt, etc)
+      <;> try { rw [beval]; rename_i H1_ih H2_ih; rw [aeval_iff_aevalR] at H1_ih; rw [aeval_iff_aevalR] at H2_ih; rw [H1_ih]; rw [H2_ih] }
+      -- base cases
+      <;> try { rfl }
+    -- 1 IH on boolean
+    rw [beval]; rename_i H1_ih; rw [H1_ih]
+    -- 2 IH on boolean
+    rw [beval]; rename_i H1_ih H2_ih; rw [H1_ih]; rw [H2_ih]; simp
+  . revert bv; induction b <;> intros b H
+      <;> try { rw [beval.eq_def] at H; simp at H; rewrite [H]; constructor }
+    case mpr.BEq a1 a2 =>
+      rw [<- H]; rw [beval]; apply bevalR.E_BEq;
+      . have aiar := aeval_iff_aevalR a1 (aeval a1); apply aiar.mpr; rfl;
+      . have aiar := aeval_iff_aevalR a2 (aeval a2); apply aiar.mpr; rfl;
+    case mpr.BNeq a1 a2 =>
+      rw [<- H]; rw [beval]; apply bevalR.E_BNeq;
+      . have aiar := aeval_iff_aevalR a1 (aeval a1); apply aiar.mpr; rfl;
+      . have aiar := aeval_iff_aevalR a2 (aeval a2); apply aiar.mpr; rfl;
+    case mpr.BLe a1 a2 =>
+      rw [<- H]; rw [beval]; apply bevalR.E_BLe;
+      . have aiar := aeval_iff_aevalR a1 (aeval a1); apply aiar.mpr; rfl;
+      . have aiar := aeval_iff_aevalR a2 (aeval a2); apply aiar.mpr; rfl;
+    case mpr.BGt a1 a2 =>
+      rw [<- H]; rw [beval]; apply bevalR.E_BGt;
+      . have aiar := aeval_iff_aevalR a1 (aeval a1); apply aiar.mpr; rfl;
+      . have aiar := aeval_iff_aevalR a2 (aeval a2); apply aiar.mpr; rfl;
+    case mpr.BNot b1 H1 =>
+      rw [<- H]; rw [beval]; apply bevalR.E_BNot; apply H1; rfl
+    case mpr.BAnd b1 b2 H1 H2 =>
+      rw [<- H]; rw [beval]; simp; apply bevalR.E_BAnd;
+      . apply H1; rfl
+      . apply H2; rfl
+
+
+
+
+end no_state
+
+namespace with_state
+
+inductive aexp where
+  | ANum (n : Nat)
+  | AId (x: String)
+  | APlus (a1 a2 : aexp)
+  | AMinus (a1 a2 : aexp)
+  | AMult (a1 a2 : aexp)
+
+inductive bexp where
+  | BTrue
+  | BFalse
+  | BEq (a1 a2 : aexp)
+  | BNeq (a1 a2 : aexp)
+  | BLe (a1 a2 : aexp)
+  | BGt (a1 a2 : aexp)
+  | BNot (b : bexp)
+  | BAnd (b1 b2 : bexp)
+
+open aexp
+
+def aeval (st: state)(a : aexp) : Nat :=
+  match a with
+  | ANum n => n
+  | AId x => st x
+  | APlus  a1 a2 => (aeval st a1) + (aeval st a2)
+  | AMinus a1 a2 => (aeval st a1) - (aeval st a2)
+  | AMult  a1 a2 => (aeval st a1) * (aeval st a2)
+
+open bexp
+def beval (st: state)(b : bexp) : Bool :=
+  match b with
+  | BTrue       => true
+  | BFalse      => false
+  | bexp.BEq a1 a2   => (aeval st a1) = (aeval st a2)
+  | BNeq a1 a2  => ¬ ((aeval st a1) = (aeval st a2))
+  | BLe a1 a2   => (aeval st a1) <= (aeval st a2)
+  | BGt a1 a2   => ¬ ((aeval st a1) <= (aeval st a2))
+  | BNot b1     => ¬ (beval st b1)
+  | BAnd b1 b2  =>  (beval st b1) ∧ (beval st b2)
+
+#eval aeval (!-> 0) (ANum  5)
+
+theorem test2: aeval (!-> 0) (APlus (ANum 2) (ANum 2)) = 4 :=
+by rfl
+
+open with_state
+inductive com : Type where
+  | CSkip
+  | CAsgn (x : String) (a : aexp)
+  | CSeq (c1 c2 : com)
+  | CIf (b : bexp) (c1 c2 : com)
+  | CWhile (b : bexp) (c : com)
+
+
+
+-- @[coercion]
+-- def AId : String → aexp := aexp.AId
+
+-- structure Rational where
+--   num : Int
+--   den : Nat
+--   inv : den ≠ 0
+
+-- instance : OfNat (Rational n) where
+--   ofNat := { num := n, den := 1, inv := by decide }
+namespace Test
+
+instance : OfNat aexp (l : Nat) where
+  ofNat := aexp.ANum n
+
+instance : Coe String aexp where
+  coe := aexp.AId
+
+-- @[coercion]
+-- def ANum : Nat → aexp := aexp.ANum
+
+notation: max "<{" e "}>" => e
+
+-- notation: max (priority := 2000) "(" x ")" => x
+
+notation: max (priority := high) x "+" y => APlus x y -- (in custom com at level 50, left associativity)
+notation: max (priority := high) x "-" y => AMinus x y  -- (in custom com at level 50, left associativity)
+notation: max (priority := high) x "*" y => AMult x y -- (in custom com at level 40, left associativity)
+-- notation: max "true'" => true -- (at level 1)
+notation: max (priority := high) "True" => BTrue -- (in custom com at level 0)
+-- notation: max "'false'" => false (at level 1)
+notation: max (priority := high) "False" => BFalse -- (in custom com at level 0)
+notation: max (priority := high) x "<=" y => BLe x y -- (in custom com at level 70, no associativity)
+notation: max (priority := high) x ">" y => BGt x y -- (in custom com at level 70, no associativity)
+notation: max (priority := high) x "=" y => BEq x y --(in custom com at level 70, no associativity)
+notation: max (priority := high) x "<>" y => BNeq x y -- (in custom com at level 70, no associativity)
+notation: max (priority := high) x "&&" y => BAnd x y -- (in custom com at level 80, left associativity)
+notation: max (priority := high) "~" b => BNot b  -- (in custom com at level 75, right associativity)
+def W : String := "W"
+def X : String := "X"
+def Y : String := "Y"
+def Z : String := "Z"
+
+end Test
+
+-- Open the custom scope for `com_scope`
+-- open_locale com_scope
+
+-- Example arithmetic and boolean expressions
+section
+open Test
+def example_aexp111 : aexp := <{(X * 2)}>
+def example_aexp : aexp := <{3 + (X * 2) }>
+def example_bexp : bexp := <{ True && ~(X <= 4) }>
+end
+
+-- Open the scope for `com_scope`
+-- open_locale com_scope
+
+-- -- Example arithmetic and boolean expressions
+-- def example_aexp : aexp := <{ 3 + (X * 2) }>
+-- def example_bexp : bexp := <{ true && ~(X <= 4) }>
+
+
+open com
+notation: max "skip" => CSkip
+notation: max x "::=" y => (CAsgn x y)
+notation: max x ";" y => (CSeq x y)
+notation: max "if" x "then" y "else" z "endL" => (CIf x y z)
+notation: max "while" x "doW" y "endL" => (CWhile x y)
+
+
+open with_state
+#eval (ANum 1)
+
+open with_state
+
+def ex_1 : com := ("Z" ::= (AId "X"))
+
+def ex_2 : com :=
+("Z" ::= (AId "X")) ;
+("Y" ::= (ANum 1)) ;
+while (BNeq (AId "Z") (ANum 0)) doW
+  ("Y" ::= (AId "Y")) ;
+  ("Y" ::= (ANum 1))
+endL
+
+def fact_in_lean : com :=
+("Z" ::= "X") ;
+("Y" ::= 1) ;
+while (BNeq (AId "Z") (ANum 0)) doW
+  ("Y" ::= "Y" * "Z") ;
+  ("Y" ::= "Z" - 1)
+endL
+
+
+-- Y := (ANum 1);
+-- while (Z != 0) doW (Y := (Y * Z)) endL
+
+
+-- notation:max "_ !->" v => (t_empty v)
+-- notation:max x "!->" v ";" m => (t_update m x v)
+
+-- def ex_map := "y" !-> 6; ("x" !-> 3; (_ !-> 0))
+
+
+end with_state
