LeanTmp/Second.lean
@@ -1,0 +1,3 @@
+import LeanTmp.Basic
+
+#eval hello
